opentheory/examples/byte.ml
@@ -11,6 +11,874 @@ export_thm byte_width_def;;
 
 logfile_end ();;
 
+(* Start of parametric theory instantiation: word *)
+
+#use "word-byte.ml";;
+
+(* word-def *)
+
+logfile "word-def";;
+
+let word_size_def = new_definition
+  `word_size = 2 EXP word_width`;;
+
+export_thm word_size_def;;
+
+let word_size_nonzero = prove
+  (`~(word_size = 0)`,
+   REWRITE_TAC [word_size_def; EXP_EQ_0] THEN
+   NUM_REDUCE_TAC);;
+
+export_thm word_size_nonzero;;
+
+(* Start of parametric theory instantiation: modular *)
+
+(* modular-mod *)
+
+let lt_word_size = new_axiom
+  `!n. n < word_size ==> n MOD word_size = n`;;
+
+let word_size_lt = new_axiom
+  `!n. n MOD word_size < word_size`;;
+
+let mod_mod_word_size = new_axiom
+  `!n. n MOD word_size MOD word_size = n MOD word_size`;;
+
+let add_mod_word_size = new_axiom
+  `!m n.
+     (m MOD word_size + n MOD word_size) MOD word_size =
+     (m + n) MOD word_size`;;
+
+let mult_mod_word_size = new_axiom
+  `!m n.
+     (m MOD word_size * n MOD word_size) MOD word_size =
+     (m * n) MOD word_size`;;
+
+(* modular-def *)
+
+new_type ("word",0);;
+
+new_constant ("word_add", `:word -> word -> word`);;
+new_constant ("word_mult", `:word -> word -> word`);;
+new_constant ("word_neg", `:word -> word`);;
+new_constant ("word_sub", `:word -> word -> word`);;
+new_constant ("word_le", `:word -> word -> bool`);;
+new_constant ("word_lt", `:word -> word -> bool`);;
+new_constant ("num_to_word", `:num -> word`);;
+new_constant ("word_to_num", `:word -> num`);;
+
+let word_to_num_to_word = new_axiom
+  `!x. num_to_word (word_to_num x) = x`;;
+
+let num_to_word_inj = new_axiom
+  `!x y.
+     x < word_size /\ y < word_size /\ num_to_word x = num_to_word y ==>
+     x = y`;;
+
+let num_to_word_to_num = new_axiom
+  `!x. word_to_num (num_to_word x) = x MOD word_size`;;
+
+let num_to_word_add = new_axiom
+  `!x1 y1.
+     num_to_word (x1 + y1) = word_add (num_to_word x1) (num_to_word y1)`;;
+
+let num_to_word_mult = new_axiom
+  `!x1 y1.
+     num_to_word (x1 * y1) = word_mult (num_to_word x1) (num_to_word y1)`;;
+
+let word_neg_def = new_axiom
+  `!x. word_neg x = num_to_word (word_size - word_to_num x)`;;
+
+let word_sub_def = new_axiom
+  `!x y. word_sub x y = word_add x (word_neg y)`;;
+
+let word_le_def = new_axiom
+  `!x y. word_le x y = word_to_num x <= word_to_num y`;;
+
+let word_lt_def = new_axiom
+  `!x y. word_lt x y = ~(word_le y x)`;;
+
+(* modular-thm *)
+
+let word_to_num_inj = new_axiom
+  `!x y. word_to_num x = word_to_num y ==> x = y`;;
+
+let num_to_word_eq = new_axiom
+  `!x y. num_to_word x = num_to_word y <=> x MOD word_size = y MOD word_size`;;
+
+let word_to_num_bound = new_axiom
+  `!x. word_to_num x < word_size`;;
+
+let word_to_num_div_bound = new_axiom
+  `!x. word_to_num x DIV word_size = 0`;;
+
+let word_add_to_num = new_axiom
+  `!x y.
+     word_to_num (word_add x y) =
+     (word_to_num x + word_to_num y) MOD word_size`;;
+
+(* End of parametric theory instantiation: modular *)
+
+logfile "word-bits-def";;
+
+let word_shl_def = new_definition
+ `!w n. word_shl w n = num_to_word ((2 EXP n) * word_to_num w)`;;
+
+export_thm word_shl_def;;
+
+let word_shr_def = new_definition
+ `!w n. word_shr w n = num_to_word (word_to_num w DIV (2 EXP n))`;;
+
+export_thm word_shr_def;;
+
+let word_bit_def = new_definition
+ `!w n. word_bit w n = ODD (word_to_num (word_shr w n))`;;
+
+export_thm word_bit_def;;
+
+let word_to_list_def = new_definition
+ `!w. word_to_list w = MAP (word_bit w) (interval 0 word_width)`;;
+
+export_thm word_to_list_def;;
+
+let list_to_word_def = new_recursive_definition list_RECURSION
+  `(list_to_word [] = num_to_word 0) /\
+   (!h t.
+      list_to_word (CONS h t) =
+      if h then word_add (word_shl (list_to_word t) 1) (num_to_word 1)
+      else word_shl (list_to_word t) 1)`;;
+
+export_thm list_to_word_def;;
+
+let is_word_list_def = new_definition
+ `!l. is_word_list (l : bool list) <=> LENGTH l = word_width`;;
+
+export_thm is_word_list_def;;
+
+let word_and_def = new_definition
+  `!w1 w2.
+     word_and w1 w2 =
+     list_to_word (zipwith ( /\ ) (word_to_list w1) (word_to_list w2))`;;
+
+export_thm word_and_def;;
+
+let word_or_def = new_definition
+  `!w1 w2.
+     word_or w1 w2 =
+     list_to_word (zipwith ( \/ ) (word_to_list w1) (word_to_list w2))`;;
+
+export_thm word_or_def;;
+
+let word_not_def = new_definition
+  `!w. word_not w = list_to_word (MAP (~) (word_to_list w))`;;
+
+export_thm word_not_def;;
+
+logfile "word-bits-thm";;
+
+(* Helper theorems (not exported) *)
+
+let even_0 = prove
+  (`!n. n = 0 ==> EVEN n`,
+   GEN_TAC THEN
+   DISCH_THEN SUBST_VAR_TAC THEN
+   REWRITE_TAC [EVEN]);;
+
+let cons_div_2 = prove
+  (`!n h. (2 * n + (if h then 1 else 0)) DIV 2 = n`,
+   REPEAT GEN_TAC THEN
+   MATCH_MP_TAC EQ_TRANS THEN
+   EXISTS_TAC `(2 * n) DIV 2 + (if h then 1 else 0) DIV 2` THEN
+   CONJ_TAC THENL
+   [MP_TAC (SPECL [`2 * n`; `if h then 1 else 0`; `2`] DIV_ADD_MOD) THEN
+    COND_TAC THENL
+    [NUM_REDUCE_TAC;
+     ALL_TAC] THEN
+    DISCH_THEN (fun th -> REWRITE_TAC [GSYM th]) THEN
+    MP_TAC (SPECL [`2`; `n : num`] MOD_MULT) THEN
+    COND_TAC THENL
+    [NUM_REDUCE_TAC;
+     ALL_TAC] THEN
+    DISCH_THEN (fun th -> REWRITE_TAC [th; ADD]) THEN
+    BOOL_CASES_TAC `h:bool` THENL
+    [REWRITE_TAC [] THEN
+     NUM_REDUCE_TAC THEN
+     REWRITE_TAC [GSYM ODD_MOD; GSYM ADD1; ODD_DOUBLE];
+     REWRITE_TAC [] THEN
+     NUM_REDUCE_TAC THEN
+     REWRITE_TAC [GSYM EVEN_MOD; ADD_0; EVEN_DOUBLE]];
+    ALL_TAC] THEN
+   MP_TAC (SPECL [`2`; `n : num`] DIV_MULT) THEN
+   COND_TAC THENL
+   [NUM_REDUCE_TAC;
+    ALL_TAC] THEN
+   DISCH_THEN (fun th -> REWRITE_TAC [th; EQ_ADD_LCANCEL_0]) THEN
+   MATCH_MP_TAC DIV_LT THEN
+   BOOL_CASES_TAC `h : bool` THEN
+   REWRITE_TAC [] THEN
+   NUM_REDUCE_TAC);;
+
+let exp_2_nz = prove
+  (`!n. ~(2 EXP n = 0)`,
+   REWRITE_TAC [EXP_EQ_0] THEN
+   NUM_REDUCE_TAC);;
+
+let le_exp_2 = prove
+  (`!m n. 2 EXP m <= 2 EXP n <=> m <= n`,
+   REWRITE_TAC [LE_EXP] THEN
+   NUM_REDUCE_TAC);;
+
+let lt_exp_2 = prove
+  (`!m n. 2 EXP m < 2 EXP n <=> m < n`,
+   REWRITE_TAC [LT_EXP] THEN
+   NUM_REDUCE_TAC);;
+
+let lt_exp_2_suc = prove
+  (`!m n. m < 2 EXP n ==> 2 * m + 1 < 2 EXP SUC n`,
+   REPEAT STRIP_TAC THEN
+   MATCH_MP_TAC LTE_TRANS THEN
+   EXISTS_TAC `2 * (m + 1)` THEN
+   CONJ_TAC THENL
+   [REWRITE_TAC [LEFT_ADD_DISTRIB; LT_ADD_LCANCEL] THEN
+    NUM_REDUCE_TAC;
+    ALL_TAC] THEN
+   REWRITE_TAC [EXP; LE_MULT_LCANCEL] THEN
+   DISJ2_TAC THEN
+   ASM_REWRITE_TAC [GSYM ADD1; LE_SUC_LT]);;
+
+let mod_exp_2_lt = prove
+  (`!m n. m MOD (2 EXP n) < 2 EXP n`,
+   REPEAT GEN_TAC THEN
+   MP_TAC (SPECL [`m : num`; `2 EXP n`] DIVISION) THEN
+   COND_TAC THENL
+   [REWRITE_TAC [exp_2_nz];
+    DISCH_THEN (fun th -> ACCEPT_TAC (CONJUNCT2 th))]);;
+
+let div_exp_2_lt = prove
+  (`!m n. m DIV (2 EXP n) = 0 <=> m < 2 EXP n`,
+   REPEAT GEN_TAC THEN
+   MATCH_MP_TAC DIV_EQ_0 THEN
+   MATCH_ACCEPT_TAC exp_2_nz);;
+
+let cond_mod_2 = prove
+  (`!n. (if ODD n then 1 else 0) = n MOD 2`,
+   GEN_TAC THEN
+   MP_TAC (SPEC `n:num` EVEN_OR_ODD) THEN
+   STRIP_TAC THENL
+   [MP_TAC (SPEC `n:num` EVEN_MOD) THEN
+    ASM_REWRITE_TAC [] THEN
+    DISCH_THEN (fun th -> REWRITE_TAC [th]) THEN
+    MP_TAC (SPEC `n:num` NOT_ODD) THEN
+    ASM_REWRITE_TAC [] THEN
+    DISCH_THEN (fun th -> REWRITE_TAC [th]);
+    MP_TAC (SPEC `n:num` ODD_MOD) THEN
+    ASM_REWRITE_TAC [] THEN
+    DISCH_THEN (fun th -> REWRITE_TAC [th])]);;
+
+let odd_mod_exp_2 = prove
+  (`!m n. ODD (m MOD (2 EXP n)) <=> ODD m /\ ~(n = 0)`,
+   REPEAT GEN_TAC THEN
+   MP_TAC (SPEC `n:num` num_CASES) THEN
+   STRIP_TAC THENL
+   [ASM_REWRITE_TAC [EXP; MULT_CLAUSES; MOD_1; ODD];
+    ALL_TAC] THEN
+   POP_ASSUM SUBST_VAR_TAC THEN
+   REWRITE_TAC [NOT_SUC; EXP; ODD_MOD] THEN
+   AP_THM_TAC THEN
+   AP_TERM_TAC THEN
+   MATCH_MP_TAC MOD_MOD THEN
+   REWRITE_TAC [GSYM EXP; exp_2_nz]);;
+
+let mod_div_exp_2 = prove
+  (`!x m n.
+      (x MOD (2 EXP m)) DIV (2 EXP n) =
+      (if m <= n then 0 else (x DIV (2 EXP n)) MOD (2 EXP (m - n)))`,
+   REPEAT GEN_TAC THEN
+   bool_cases_tac `m <= n` THENL
+   [ASM_REWRITE_TAC [] THEN
+    MATCH_MP_TAC DIV_LT THEN
+    MATCH_MP_TAC LTE_TRANS THEN
+    EXISTS_TAC `2 EXP m` THEN
+    ASM_REWRITE_TAC [le_exp_2; mod_exp_2_lt];
+    ALL_TAC] THEN
+   ASM_REWRITE_TAC [] THEN
+   MP_TAC (SPECL [`x : num`; `2 EXP n`; `2 EXP (m - n)`] DIV_MOD) THEN
+   COND_TAC THENL
+   [REWRITE_TAC [MULT_EQ_0; exp_2_nz];
+    ALL_TAC] THEN
+   DISCH_THEN (fun th -> REWRITE_TAC [th]) THEN
+   AP_THM_TAC THEN
+   AP_TERM_TAC THEN
+   AP_TERM_TAC THEN
+   REWRITE_TAC [GSYM EXP_ADD] THEN
+   AP_TERM_TAC THEN
+   ASM_ARITH_TAC);;
+
+(* Exported theorems *)
+
+let length_word_to_list = prove
+  (`!w. LENGTH (word_to_list w) = word_width`,
+   REWRITE_TAC [word_to_list_def; LENGTH_MAP; length_interval]);;
+
+export_thm length_word_to_list;;
+
+let is_word_to_list = prove
+  (`!w. is_word_list (word_to_list w)`,
+   REWRITE_TAC [is_word_list_def; length_word_to_list]);;
+
+export_thm is_word_to_list;;
+
+let word_bit_div = prove
+  (`!w n. word_bit w n = ODD (word_to_num w DIV (2 EXP n))`,
+   REWRITE_TAC [word_bit_def; word_shr_def; num_to_word_to_num] THEN
+   REPEAT GEN_TAC THEN
+   AP_TERM_TAC THEN
+   MATCH_MP_TAC lt_word_size THEN
+   MATCH_MP_TAC LET_TRANS THEN
+   EXISTS_TAC `word_to_num w` THEN
+   CONJ_TAC THENL
+   [MATCH_MP_TAC DIV_LE THEN
+    REWRITE_TAC [EXP_EQ_0] THEN
+    NUM_REDUCE_TAC;
+    REWRITE_TAC [word_to_num_bound]]);;
+
+export_thm word_bit_div;;
+
+let nil_to_word_to_num = prove
+  (`word_to_num (list_to_word []) = 0`,
+   REWRITE_TAC [list_to_word_def; num_to_word_to_num] THEN
+   MATCH_MP_TAC lt_word_size THEN
+   REWRITE_TAC [LT_NZ; word_size_nonzero]);;
+
+export_thm nil_to_word_to_num;;
+
+let cons_to_word_to_num = prove
+  (`!h t.
+      word_to_num (list_to_word (CONS h t)) =
+      (2 * word_to_num (list_to_word t) + (if h then 1 else 0)) MOD word_size`,
+   REWRITE_TAC [list_to_word_def] THEN
+   REPEAT STRIP_TAC THEN
+   MP_TAC (SPEC `h : bool` BOOL_CASES_AX) THEN
+   STRIP_TAC THENL
+   [ASM_REWRITE_TAC
+      [word_add_to_num; word_shl_def; EXP_1; word_to_num_to_word] THEN
+    REWRITE_TAC [num_to_word_to_num; add_mod_word_size];
+    ASM_REWRITE_TAC [word_shl_def; EXP_1; word_to_num_to_word; ADD_0] THEN
+    REWRITE_TAC [num_to_word_to_num; add_mod_word_size]]);;
+
+export_thm cons_to_word_to_num;;
+
+let list_to_word_to_num_bound = prove
+  (`!l. word_to_num (list_to_word l) < 2 EXP (LENGTH l)`,
+   LIST_INDUCT_TAC THENL
+   [REWRITE_TAC [nil_to_word_to_num; LENGTH; EXP] THEN
+    NUM_REDUCE_TAC;
+    ALL_TAC] THEN
+   REWRITE_TAC [cons_to_word_to_num; LENGTH] THEN
+   MATCH_MP_TAC LET_TRANS THEN
+   EXISTS_TAC `2 * word_to_num (list_to_word t) + (if h then 1 else 0)` THEN
+   CONJ_TAC THENL
+   [MATCH_MP_TAC MOD_LE THEN
+    ACCEPT_TAC word_size_nonzero;
+    ALL_TAC] THEN
+   MATCH_MP_TAC LET_TRANS THEN
+   EXISTS_TAC `2 * word_to_num (list_to_word t) + 1` THEN
+   CONJ_TAC THENL
+   [REWRITE_TAC [LE_ADD_LCANCEL] THEN
+    BOOL_CASES_TAC `h : bool`THEN
+    REWRITE_TAC [LE_REFL] THEN
+    NUM_REDUCE_TAC;
+    ALL_TAC] THEN
+   MATCH_MP_TAC lt_exp_2_suc THEN
+   FIRST_ASSUM ACCEPT_TAC);;
+
+export_thm list_to_word_to_num_bound;;
+
+let list_to_word_to_num_bound_suc = prove
+  (`!l. 2 * word_to_num (list_to_word l) + 1 < 2 EXP (SUC (LENGTH l))`,
+   GEN_TAC THEN
+   MATCH_MP_TAC lt_exp_2_suc THEN
+   MATCH_ACCEPT_TAC list_to_word_to_num_bound);;
+
+export_thm list_to_word_to_num_bound_suc;;
+
+let cons_to_word_to_num_bound = prove
+  (`!h t.
+      2 * word_to_num (list_to_word t) + (if h then 1 else 0) <
+      2 EXP SUC (LENGTH t)`,
+   REPEAT GEN_TAC THEN
+   MATCH_MP_TAC LET_TRANS THEN
+   EXISTS_TAC `2 * word_to_num (list_to_word t) + 1` THEN
+   CONJ_TAC THENL
+   [REWRITE_TAC [LE_ADD_LCANCEL] THEN
+    BOOL_CASES_TAC `h : bool` THEN
+    REWRITE_TAC [LE_REFL; LE_0];
+    MATCH_ACCEPT_TAC list_to_word_to_num_bound_suc]);;
+
+export_thm cons_to_word_to_num_bound;;
+
+let word_to_list_to_word = prove
+  (`!w. list_to_word (word_to_list w) = w`,
+   GEN_TAC THEN
+   REWRITE_TAC [word_to_list_def] THEN
+   MATCH_MP_TAC word_to_num_inj THEN
+   MATCH_MP_TAC (ITAUT`!p q. (p ==> q) /\ p ==> q`) THEN
+   EXISTS_TAC
+     `!k.
+        k <= word_width ==>
+        word_to_num
+          (list_to_word (MAP (word_bit w) (interval (word_width - k) k))) =
+          word_to_num w DIV (2 EXP (word_width - k))` THEN
+   CONJ_TAC THENL
+   [DISCH_THEN (MP_TAC o SPEC `word_width`) THEN
+    REWRITE_TAC [SUB_REFL; LE_REFL; EXP; DIV_1];
+    ALL_TAC] THEN
+   MATCH_MP_TAC num_INDUCTION THEN
+   CONJ_TAC THENL
+   [REWRITE_TAC
+      [SUB; interval_def; MAP; nil_to_word_to_num; GSYM word_size_def;
+       word_to_num_div_bound];
+    ALL_TAC] THEN
+   REPEAT STRIP_TAC THEN
+   PAT_ASSUM `X ==> Y` THEN
+   MATCH_MP_TAC (ITAUT `X /\ (Y ==> Z) ==> ((X ==> Y) ==> Z)`) THEN
+   CONJ_TAC THENL
+   [MATCH_MP_TAC LE_TRANS THEN
+    EXISTS_TAC `SUC k` THEN
+    ASM_REWRITE_TAC [LE; LE_REFL];
+    ALL_TAC] THEN
+   REWRITE_TAC [interval_def; MAP; cons_to_word_to_num] THEN
+   KNOW_TAC `word_width - k = SUC (word_width - SUC k)` THENL
+   [ASM_ARITH_TAC;
+    ALL_TAC] THEN
+   DISCH_THEN (fun th -> REWRITE_TAC [th]) THEN
+   DISCH_THEN (fun th -> REWRITE_TAC [th]) THEN
+   REWRITE_TAC [word_bit_div; cond_mod_2] THEN
+   ONCE_REWRITE_TAC [MULT_SYM] THEN
+   REWRITE_TAC [EXP] THEN
+   MP_TAC (SPECL [`word_to_num w`; `2 EXP (word_width - SUC k)`;
+                   `2`] (ONCE_REWRITE_RULE [MULT_SYM] DIV_DIV)) THEN
+   MATCH_MP_TAC (ITAUT `X /\ (Y ==> Z) ==> ((X ==> Y) ==> Z)`) THEN
+   CONJ_TAC THENL
+   [REWRITE_TAC [GSYM EXP; EXP_EQ_0] THEN
+    NUM_REDUCE_TAC;
+    ALL_TAC] THEN
+   DISCH_THEN (fun th -> REWRITE_TAC [GSYM th]) THEN
+   MP_TAC (SPECL [`word_to_num w DIV (2 EXP (word_width - SUC k))`;
+                   `2`] DIVISION) THEN
+   MATCH_MP_TAC (ITAUT `X /\ (Y ==> Z) ==> ((X ==> Y) ==> Z)`) THEN
+   CONJ_TAC THENL
+   [NUM_REDUCE_TAC;
+    ALL_TAC] THEN
+   DISCH_THEN (fun th -> REWRITE_TAC [GSYM (CONJUNCT1 th)]) THEN
+   MATCH_MP_TAC lt_word_size THEN
+   MATCH_MP_TAC LET_TRANS THEN
+   EXISTS_TAC `word_to_num w` THEN
+   CONJ_TAC THENL
+   [MATCH_MP_TAC DIV_LE THEN
+    REWRITE_TAC [EXP_EQ_0] THEN
+    NUM_REDUCE_TAC;
+    REWRITE_TAC [word_to_num_bound]]);;
+
+export_thm word_to_list_to_word;;
+
+let word_to_list_inj = prove
+  (`!w1 w2. word_to_list w1 = word_to_list w2 ==> w1 = w2`,
+   REPEAT STRIP_TAC THEN
+   ONCE_REWRITE_TAC [GSYM word_to_list_to_word] THEN
+   ASM_REWRITE_TAC []);;
+
+export_thm word_to_list_inj;;
+
+let list_to_word_bit = prove
+  (`!l n.
+      word_bit (list_to_word l) n =
+      (n < word_width /\ n < LENGTH l /\ EL n l)`,
+   REWRITE_TAC [word_bit_div] THEN
+   ONCE_REWRITE_TAC [SWAP_FORALL_THM] THEN
+   MATCH_MP_TAC num_INDUCTION THEN
+   CONJ_TAC THENL
+   [LIST_INDUCT_TAC THENL
+    [REWRITE_TAC [LENGTH; nil_to_word_to_num; LT; ODD; EXP; DIV_1];
+     ALL_TAC] THEN
+    POP_ASSUM (K ALL_TAC) THEN
+    REWRITE_TAC
+      [LENGTH; cons_to_word_to_num; EXP; DIV_1; EL; HD; LT_NZ; NOT_SUC] THEN
+    ASM_REWRITE_TAC [word_size_def; odd_mod_exp_2] THEN
+    CONV_TAC (RATOR_CONV (ONCE_REWRITE_CONV [CONJ_SYM])) THEN
+    AP_TERM_TAC THEN
+    MP_TAC (SPEC `h:bool` BOOL_CASES_AX) THEN
+    STRIP_TAC THENL
+    [ASM_REWRITE_TAC [GSYM ADD1; ODD_DOUBLE];
+     ASM_REWRITE_TAC [ADD_0; GSYM NOT_EVEN; EVEN_DOUBLE]];
+    ALL_TAC] THEN
+   GEN_TAC THEN
+   STRIP_TAC THEN
+   bool_cases_tac' `SUC n < word_width` THENL
+   [POP_ASSUM MP_TAC THEN
+    POP_ASSUM (K ALL_TAC) THEN
+    REPEAT STRIP_TAC THEN
+    ASM_REWRITE_TAC [NOT_ODD] THEN
+    MATCH_MP_TAC even_0 THEN
+    REWRITE_TAC [div_exp_2_lt] THEN
+    MATCH_MP_TAC LTE_TRANS THEN
+    EXISTS_TAC `word_size` THEN
+    REWRITE_TAC [word_to_num_bound] THEN
+    REWRITE_TAC [word_size_def; le_exp_2] THEN
+    ASM_ARITH_TAC;
+    ALL_TAC] THEN
+   ASM_REWRITE_TAC [] THEN
+   LIST_INDUCT_TAC THENL
+   [REWRITE_TAC [LENGTH; nil_to_word_to_num; LT; NOT_ODD] THEN
+    MATCH_MP_TAC even_0 THEN
+    REWRITE_TAC [div_exp_2_lt; LT_NZ; exp_2_nz];
+    ALL_TAC] THEN
+   POP_ASSUM (K ALL_TAC) THEN
+   REWRITE_TAC [LENGTH; cons_to_word_to_num] THEN
+   REWRITE_TAC [LT_SUC; EL; TL] THEN
+   REWRITE_TAC [word_size_def; mod_div_exp_2; GSYM NOT_LT] THEN
+   ASM_REWRITE_TAC [odd_mod_exp_2; SUB_EQ_0; GSYM NOT_LT] THEN
+   FIRST_X_ASSUM (fun th -> MP_TAC (SPEC `t : bool list` th)) THEN
+   KNOW_TAC `n < word_width` THENL
+   [ASM_ARITH_TAC;
+    ALL_TAC] THEN
+   DISCH_THEN (fun th -> REWRITE_TAC [th]) THEN
+   DISCH_THEN (fun th -> REWRITE_TAC [GSYM th]) THEN
+   REWRITE_TAC [ODD_MOD] THEN
+   AP_THM_TAC THEN
+   AP_TERM_TAC THEN
+   AP_THM_TAC THEN
+   AP_TERM_TAC THEN
+   MATCH_MP_TAC EQ_TRANS THEN
+   EXISTS_TAC
+     `((2 * word_to_num (list_to_word t) + (if h then 1 else 0)) DIV 2) DIV
+      (2 EXP n)` THEN
+   CONJ_TAC THENL
+   [REWRITE_TAC [EXP] THEN
+    MATCH_MP_TAC EQ_SYM THEN
+    MATCH_MP_TAC DIV_DIV THEN
+    REWRITE_TAC [GSYM EXP; exp_2_nz];
+    ALL_TAC] THEN
+   AP_THM_TAC THEN
+   AP_TERM_TAC THEN
+   MATCH_ACCEPT_TAC cons_div_2);;
+
+export_thm list_to_word_bit;;
+
+let short_list_to_word_to_list = prove
+  (`!l.
+      LENGTH l <= word_width ==>
+      word_to_list (list_to_word l) =
+      APPEND l (REPLICATE (word_width - LENGTH l) F)`,
+   REWRITE_TAC [word_to_list_def; list_to_word_bit] THEN
+   REPEAT STRIP_TAC THEN
+   MATCH_MP_TAC nth_eq THEN
+   REWRITE_TAC [LENGTH_MAP; length_interval] THEN
+   CONJ_TAC THENL
+   [REWRITE_TAC [LENGTH_APPEND; LENGTH_REPLICATE] THEN
+    ASM_ARITH_TAC;
+    ALL_TAC] THEN
+   REPEAT STRIP_TAC THEN
+   MP_TAC (ISPECL [`word_bit (list_to_word l)`; `interval 0 word_width`;
+                   `i : num`] nth_map) THEN
+   COND_TAC THENL
+   [ASM_REWRITE_TAC [length_interval];
+    ALL_TAC] THEN
+   DISCH_THEN (fun th -> REWRITE_TAC [th]) THEN
+   MP_TAC (SPECL [`0`; `word_width`; `i : num`] nth_interval) THEN
+   ASM_REWRITE_TAC [ADD] THEN
+   DISCH_THEN (fun th -> REWRITE_TAC [th]) THEN
+   REWRITE_TAC [list_to_word_bit] THEN
+   ASM_REWRITE_TAC [EL_APPEND] THEN
+   bool_cases_tac `i < LENGTH (l : bool list)` THENL
+   [ASM_REWRITE_TAC [];
+    ALL_TAC] THEN
+   ASM_REWRITE_TAC [] THEN
+   MP_TAC (ISPECL [`word_width - LENGTH (l : bool list)`; `F`;
+                   `i - LENGTH (l : bool list)`] nth_replicate) THEN
+   COND_TAC THENL
+   [ASM_ARITH_TAC;
+    DISCH_THEN (fun th -> REWRITE_TAC [th])]);;
+
+export_thm short_list_to_word_to_list;;
+
+let long_list_to_word_to_list = prove
+  (`!l.
+      word_width <= LENGTH l ==>
+      word_to_list (list_to_word l) = take word_width l`,
+   REWRITE_TAC [word_to_list_def; list_to_word_bit] THEN
+   REPEAT STRIP_TAC THEN
+   MATCH_MP_TAC nth_eq THEN
+   REWRITE_TAC [LENGTH_MAP; length_interval] THEN
+   CONJ_TAC THENL
+   [MATCH_MP_TAC EQ_SYM THEN
+    MATCH_MP_TAC length_take THEN
+    FIRST_ASSUM ACCEPT_TAC;
+    ALL_TAC] THEN
+   REPEAT STRIP_TAC THEN
+   MP_TAC (ISPECL [`word_bit (list_to_word l)`; `interval 0 word_width`;
+                   `i : num`] nth_map) THEN
+   COND_TAC THENL
+   [ASM_REWRITE_TAC [length_interval];
+    ALL_TAC] THEN
+   DISCH_THEN (fun th -> REWRITE_TAC [th]) THEN
+   MP_TAC (SPECL [`0`; `word_width`; `i : num`] nth_interval) THEN
+   ASM_REWRITE_TAC [ADD] THEN
+   DISCH_THEN (fun th -> REWRITE_TAC [th]) THEN
+   REWRITE_TAC [list_to_word_bit] THEN
+   ASM_REWRITE_TAC [] THEN
+   KNOW_TAC `i < LENGTH (l : bool list)` THENL
+   [ASM_ARITH_TAC;
+    ALL_TAC] THEN
+   STRIP_TAC THEN
+   ASM_REWRITE_TAC [] THEN
+   MATCH_MP_TAC EQ_SYM THEN
+   MATCH_MP_TAC nth_take THEN
+   ASM_REWRITE_TAC []);;
+
+export_thm long_list_to_word_to_list;;
+
+let list_to_word_to_list_eq = prove
+  (`!l.
+      word_to_list (list_to_word l) =
+      if LENGTH l <= word_width then
+        APPEND l (REPLICATE (word_width - LENGTH l) F)
+      else
+        take word_width l`,
+   GEN_TAC THEN
+   bool_cases_tac `LENGTH (l : bool list) <= word_width` THENL
+   [ASM_REWRITE_TAC [] THEN
+    MATCH_MP_TAC short_list_to_word_to_list THEN
+    FIRST_ASSUM ACCEPT_TAC;
+    ASM_REWRITE_TAC [] THEN
+    MATCH_MP_TAC long_list_to_word_to_list THEN
+    ASM_ARITH_TAC]);;
+
+export_thm list_to_word_to_list_eq;;
+
+let list_to_word_to_list = prove
+  (`!l. LENGTH l = word_width <=> word_to_list (list_to_word l) = l`,
+   GEN_TAC THEN
+   EQ_TAC THENL
+   [STRIP_TAC THEN
+    MATCH_MP_TAC EQ_TRANS THEN
+    EXISTS_TAC `take (LENGTH (l : bool list)) l` THEN
+    CONJ_TAC THENL
+    [ASM_REWRITE_TAC [] THEN
+     MATCH_MP_TAC long_list_to_word_to_list THEN
+     ASM_REWRITE_TAC [LE_REFL];
+     MATCH_ACCEPT_TAC take_length];
+    DISCH_THEN (fun th -> ONCE_REWRITE_TAC [GSYM th]) THEN
+    MATCH_ACCEPT_TAC length_word_to_list]);;
+
+export_thm list_to_word_to_list;;
+
+let word_shl_list = prove
+  (`!l n.
+      word_shl (list_to_word l) n =
+      list_to_word (APPEND (REPLICATE n F) l)`,
+   REWRITE_TAC [word_shl_def] THEN
+   REPEAT GEN_TAC THEN
+   MATCH_MP_TAC word_to_num_inj THEN
+   REWRITE_TAC [num_to_word_to_num] THEN
+   SPEC_TAC (`n:num`,`n:num`) THEN
+   MATCH_MP_TAC num_INDUCTION THEN
+   CONJ_TAC THENL
+   [REWRITE_TAC [EXP; REPLICATE; APPEND; MULT_CLAUSES] THEN
+    REWRITE_TAC [GSYM num_to_word_to_num; word_to_num_to_word];
+    ALL_TAC] THEN
+   REPEAT STRIP_TAC THEN
+   REWRITE_TAC [REPLICATE; APPEND; cons_to_word_to_num; ADD_0] THEN
+   POP_ASSUM (fun th -> REWRITE_TAC [GSYM th]) THEN
+   MP_TAC (SPECL [`2`; `word_size`; `2 EXP n * word_to_num (list_to_word l)`]
+                 MOD_MULT_RMOD) THEN
+   COND_TAC THENL
+   [ACCEPT_TAC word_size_nonzero;
+    ALL_TAC] THEN
+   DISCH_THEN (fun th -> REWRITE_TAC [th]) THEN
+   REWRITE_TAC [EXP; MULT_ASSOC]);;
+
+export_thm word_shl_list;;
+
+let short_word_shr_list = prove
+  (`!l n.
+      LENGTH l <= word_width ==>
+      word_shr (list_to_word l) n =
+      (if LENGTH l <= n then list_to_word []
+       else list_to_word (drop n l))`,
+   REWRITE_TAC [word_shr_def] THEN
+   REPEAT STRIP_TAC THEN
+   MATCH_MP_TAC word_to_num_inj THEN
+   REWRITE_TAC [num_to_word_to_num] THEN
+   bool_cases_tac `LENGTH (l : bool list) <= n` THENL
+   [ASM_REWRITE_TAC [] THEN
+    REWRITE_TAC [nil_to_word_to_num] THEN
+    MP_TAC (SPEC `word_size` MOD_0) THEN
+    COND_TAC THENL
+    [ACCEPT_TAC word_size_nonzero;
+     ALL_TAC] THEN
+    DISCH_THEN (fun th -> ONCE_REWRITE_TAC [GSYM th]) THEN
+    AP_THM_TAC THEN
+    AP_TERM_TAC THEN
+    MATCH_MP_TAC DIV_LT THEN
+    MATCH_MP_TAC LTE_TRANS THEN
+    EXISTS_TAC `2 EXP LENGTH (l : bool list)` THEN
+    CONJ_TAC THENL
+    [MATCH_ACCEPT_TAC list_to_word_to_num_bound;
+     ALL_TAC] THEN
+    ASM_REWRITE_TAC [LE_EXP] THEN
+    NUM_REDUCE_TAC;
+    ALL_TAC] THEN
+   ASM_REWRITE_TAC [] THEN
+   KNOW_TAC `n <= LENGTH (l : bool list)` THENL
+   [ASM_ARITH_TAC;
+    ALL_TAC] THEN
+   POP_ASSUM (K ALL_TAC) THEN
+   POP_ASSUM MP_TAC THEN
+   SPEC_TAC (`n:num`,`n:num`) THEN
+   SPEC_TAC (`l : bool list`,`l : bool list`) THEN
+   LIST_INDUCT_TAC THENL
+   [REWRITE_TAC [LE; LENGTH] THEN
+    REPEAT STRIP_TAC THEN
+    ASM_REWRITE_TAC [nil_to_word_to_num; drop_def] THEN
+    NUM_REDUCE_TAC THEN
+    MATCH_MP_TAC MOD_0 THEN
+    ACCEPT_TAC word_size_nonzero;
+    ALL_TAC] THEN
+   GEN_TAC THEN
+   MP_TAC (SPEC `n : num` num_CASES) THEN
+   STRIP_TAC THENL
+   [DISCH_THEN (K ALL_TAC) THEN
+    DISCH_THEN (K ALL_TAC) THEN
+    ASM_REWRITE_TAC [EXP; DIV_1; drop_def] THEN
+    MATCH_MP_TAC MOD_LT THEN
+    MATCH_ACCEPT_TAC word_to_num_bound;
+    ALL_TAC] THEN
+   POP_ASSUM SUBST_VAR_TAC THEN
+   REWRITE_TAC [LENGTH; LE_SUC; cons_to_word_to_num; drop_def] THEN
+   REPEAT STRIP_TAC THEN
+   FIRST_X_ASSUM (fun th -> MP_TAC (SPEC `n' : num` th)) THEN
+   COND_TAC THENL
+   [ASM_ARITH_TAC;
+    ALL_TAC] THEN
+   COND_TAC THENL
+   [FIRST_ASSUM ACCEPT_TAC;
+    ALL_TAC] THEN
+   DISCH_THEN (fun th -> REWRITE_TAC [GSYM th]) THEN
+   AP_THM_TAC THEN
+   AP_TERM_TAC THEN
+   MATCH_MP_TAC EQ_TRANS THEN
+   EXISTS_TAC
+     `(2 * word_to_num (list_to_word t) + (if h then 1 else 0)) DIV
+      (2 EXP SUC n')` THEN
+   CONJ_TAC THENL
+   [AP_THM_TAC THEN
+    AP_TERM_TAC THEN
+    MATCH_MP_TAC MOD_LT THEN
+    MATCH_MP_TAC LTE_TRANS THEN
+    EXISTS_TAC `2 EXP SUC (LENGTH (t : bool list))` THEN
+    CONJ_TAC THENL
+    [MATCH_ACCEPT_TAC cons_to_word_to_num_bound;
+     ALL_TAC] THEN
+    ASM_REWRITE_TAC [word_size_def; le_exp_2];
+    ALL_TAC] THEN
+   MATCH_MP_TAC EQ_TRANS THEN
+   EXISTS_TAC
+     `((2 * word_to_num (list_to_word t) + (if h then 1 else 0)) DIV 2) DIV
+      (2 EXP n')` THEN
+   CONJ_TAC THENL
+   [REWRITE_TAC [EXP] THEN
+    MATCH_MP_TAC EQ_SYM THEN
+    MATCH_MP_TAC DIV_DIV THEN
+    REWRITE_TAC [GSYM EXP; exp_2_nz];
+    ALL_TAC] THEN
+   AP_THM_TAC THEN
+   AP_TERM_TAC THEN
+   MATCH_ACCEPT_TAC cons_div_2);;
+
+export_thm short_word_shr_list;;
+
+let long_word_shr_list = prove
+  (`!l n.
+      word_width <= LENGTH l ==>
+      word_shr (list_to_word l) n =
+      if word_width <= n then list_to_word []
+      else list_to_word (drop n (take word_width l))`,
+   REPEAT STRIP_TAC THEN
+   MP_TAC (SPEC `l : bool list` long_list_to_word_to_list) THEN
+   COND_TAC THENL
+   [FIRST_ASSUM ACCEPT_TAC;
+    ALL_TAC] THEN
+   DISCH_THEN (fun th -> REWRITE_TAC [GSYM th]) THEN
+   CONV_TAC
+     (LAND_CONV
+        (LAND_CONV (ONCE_REWRITE_CONV [GSYM word_to_list_to_word]))) THEN
+   MP_TAC (SPEC `list_to_word l` length_word_to_list) THEN
+   DISCH_THEN (fun th -> REWRITE_TAC [GSYM th] THEN ASSUME_TAC th) THEN
+   MATCH_MP_TAC short_word_shr_list THEN
+   ASM_REWRITE_TAC [LE_REFL]);;
+
+export_thm long_word_shr_list;;
+
+let word_shr_list = prove
+  (`!l n.
+      word_shr (list_to_word l) n =
+      (if LENGTH l <= word_width then
+         if LENGTH l <= n then list_to_word []
+         else list_to_word (drop n l)
+       else
+         if word_width <= n then list_to_word []
+         else list_to_word (drop n (take word_width l)))`,
+   REPEAT GEN_TAC THEN
+   bool_cases_tac `LENGTH (l : bool list) <= word_width` THENL
+   [ASM_REWRITE_TAC [] THEN
+    MATCH_MP_TAC short_word_shr_list THEN
+    FIRST_ASSUM ACCEPT_TAC;
+    ASM_REWRITE_TAC [] THEN
+    MATCH_MP_TAC long_word_shr_list THEN
+    ASM_ARITH_TAC]);;
+
+export_thm word_shr_list;;
+
+let word_eq_bits = prove
+  (`!w1 w2. (!i. i < word_width ==> word_bit w1 i = word_bit w2 i) ==> w1 = w2`,
+   REPEAT GEN_TAC THEN
+   CONV_TAC (LAND_CONV (ONCE_REWRITE_CONV [GSYM word_to_list_to_word])) THEN
+   REWRITE_TAC [list_to_word_bit] THEN
+   STRIP_TAC THEN
+   MATCH_MP_TAC word_to_list_inj THEN
+   MATCH_MP_TAC nth_eq THEN
+   REWRITE_TAC [length_word_to_list] THEN
+   REPEAT STRIP_TAC THEN
+   FIRST_X_ASSUM (fun th -> MP_TAC (SPEC `i : num` th)) THEN
+   ASM_REWRITE_TAC [length_word_to_list]);;
+
+export_thm word_eq_bits;;
+
+(***
+let num_to_word_list = prove
+  (`(num_to_word 0 = list_to_word []) /\
+    (!n. num_to_word n = list_to_word []) /\
+
+let num_to_word_list = prove
+  (`(num_to_word 0 = list_to_word []) /\
+    (!n. num_to_word n = list_to_word []) /\
+
+word_and (list_to_word []) l2 = list_to_word []) /\
+    (!l1. word_and l1 (list_to_word []) = list_to_word []) /\
+    (!h1 t1 h2 t2.
+
+let word_and_list = prove
+  (`(!l2. word_and (list_to_word []) l2 = list_to_word []) /\
+    (!l1. word_and l1 (list_to_word []) = list_to_word []) /\
+    (!h1 t1 h2 t2.
+       word_and (list_to_word (CONS h1 t1)) (list_to_word (CONS h2 t2)) =
+       list_to_word (CONS (h1 /\ h2) (word_to_list (word_and (list_to_word t1) (CONS h1 t1)) (list_to_word (CONS h2 t2)) =
+!w1 w2.
+     word_and w1 w2 =
+     list_to_word (zipwith ( /\ ) (word_to_list w1) (word_to_list w2))`;;
+***)
+
 (* Apply theory functor word *)
 
 new_type ("byte",0);;
